
Similarly, as $y \to \Im(z)$, the vertical integral of $f$ from $z$ to $\Re(z)+iy$ is equal to
$(y - \Im(z)) f(z)$, up to $o(y - \Im(z))$.
\begin{lemma}
  \label{deriv_of_wedgeInt_im'}
  \lean{deriv_of_wedgeInt_im'}\leanok
  As $y \to \Im(z)$,
  $$
    \int_{\Im(z)}^y f(\Re(z)+it)\ dt
    =
    (y-\Im(z)) f(z)
    +
    o(y-\Im(z))
    .
  $$
\end{lemma}
The proof is the same.



As before, we extend this to the setting where $w$ is in a neighborhood of $z$.
\begin{lemma}
  \label{deriv_of_wedgeInt_im''}
  \lean{deriv_of_wedgeInt_im''}\leanok
  As $w \to z$,
  $$
    \int_{\Im(z)}^{\Im(w)} f(\Re(z)+iy)\ dy
    =
    (\Im(w-z)) f(z)
    +
    o(w-z)
    .
  $$
\end{lemma}
The proof is again the same


